LoCalSyntax.v
@@ -63,6 +63,37 @@ Record program : Type := Program
     prog_fdecls : list fdecl;
     prog_main : expr }.
 
+(* ================================================================= *)
+(* Decidable equality for all identifier types                        *)
+(* ================================================================= *)
+
+Lemma tycon_eq_dec : forall (a b : tycon), {a = b} + {a <> b}.
+Proof. decide equality; apply string_dec. Defined.
+
+Lemma datacon_eq_dec : forall (a b : datacon), {a = b} + {a <> b}.
+Proof. decide equality; apply string_dec. Defined.
+
+Lemma fun_var_eq_dec : forall (a b : fun_var), {a = b} + {a <> b}.
+Proof. decide equality; apply string_dec. Defined.
+
+Lemma term_var_eq_dec : forall (a b : term_var), {a = b} + {a <> b}.
+Proof. decide equality; apply string_dec. Defined.
+
+Lemma loc_var_eq_dec : forall (a b : loc_var), {a = b} + {a <> b}.
+Proof. decide equality; apply string_dec. Defined.
+
+Lemma region_var_eq_dec : forall (a b : region_var), {a = b} + {a <> b}.
+Proof. decide equality; apply string_dec. Defined.
+
+(* Symbolic location address: a (loc_var, region_var) pair. *)
+Definition laddr : Type := (loc_var * region_var)%type.
+
+Lemma laddr_eq_dec : forall (a b : laddr), {a = b} + {a <> b}.
+Proof. decide equality; [apply region_var_eq_dec | apply loc_var_eq_dec]. Defined.
+
+(* Datacon info: maps constructor names to (result tycon, field tycons). *)
+Definition datacon_info : Type := list (datacon * (tycon * list tycon)).
+
 Declare Custom Entry local_ty.
 Declare Custom Entry local_val.
 Declare Custom Entry local_exp.
